Major def changes toward is_step_correct with app.
* Dataflow: introduce sem_node.
* Minimp: (re-)implement step and reset.
* Minimp: change the class mechanism.
* 'held semantics': start rationalizing (less rafistolage!).
* Translation: better handling of step and reset.
* Remove several admits for EqApp.

* Is_step_correct is now broken, but the new definitions should allow
  for a new invariant that includes EqApp.

Minimp.v
@@ -17,69 +17,61 @@ Inductive stmt : Set :=
   | Assign : ident -> exp -> stmt
   | AssignSt : ident -> exp -> stmt
   | Ifte : exp -> stmt -> stmt -> stmt
-  | Step_ap : ident -> ident -> exp -> stmt
+  | Step_ap : ident -> ident -> ident -> exp -> stmt
+           (* y = Step_ap class object arg *)
+  | Reset_ap : ident -> ident -> stmt
+           (* Reset_ap class object *)
   | Comp : stmt -> stmt -> stmt
   | Skip.
 
 Record obj_dec : Set := mk_obj_dec {
-  obj_name : ident;
-  obj_value : ident
+  obj_inst  : ident;
+  obj_class : ident
 }.
 
-Record step_fun : Set := mk_step_fun {
-  input : ident;
-  output : ident;
-  locals : list ident;
-  body : stmt
+Record class : Set := mk_class {
+  c_name   : ident;
+
+  c_input  : ident;
+  c_output : ident;
+
+  c_mems   : list ident;       (* TODO: should track type of each *)
+  c_objs   : list obj_dec;
+
+  c_step   : stmt;
+  c_reset  : stmt
 }.
 
-Record class_def : Set := mk_class {
-  c_id : ident;
-  c_objs : list obj_dec;
-  c_step : step_fun
-}.
+Definition program : Type := list class.
 
-Definition program : Type := list class_def.
+Definition find_class (n: ident) : program -> option class :=
+  List.find (fun c=> ident_eqb c.(c_name) n).
 
 (** ** Semantics *)
 
-(* TODO: I never seem to use/need machines and global
-environment. Joperationnal.v doesn't seem use them either. Yet, that's
-disturbing: where are the compiled ojects, in the memory env?
-
-Record machine : Set :=
-  mk_machine {
-      m_instances: PositiveMap.t ident;
-      m_step: step_fun
-    }.
-
-Definition globalEnv : Set := PositiveMap.t machine.
- *)
-
-Record memoryEnv : Set :=
-  mk_memory {
-      m_values : PM.t const;
-      m_instances : PM.t step_fun
-    }.
+Inductive memoryEnv : Set :=
+  mk_memory
+    { m_values  : PM.t const;
+      m_objects : PM.t memoryEnv }.
 
 Definition add_mem (id: ident) (v: const) (menv: memoryEnv) : memoryEnv :=
   mk_memory (PM.add id v menv.(m_values))
-            (menv.(m_instances)).
+            (menv.(m_objects)).
 
 Definition find_mem (id: ident) (menv: memoryEnv) : option const :=
   PM.find id (menv.(m_values)).
 
-Definition add_object (id: ident) (f: step_fun) (menv: memoryEnv) : memoryEnv :=
-  mk_memory menv.(m_values)
-            (PM.add id f menv.(m_instances)).
+Definition add_obj (id: ident) (omenv: memoryEnv) (menv: memoryEnv)
+  : memoryEnv := mk_memory menv.(m_values)
+                           (PM.add id omenv menv.(m_objects)).
 
-Definition find_object (id: ident) (menv: memoryEnv) : option step_fun :=
-  PM.find id (menv.(m_instances)).
-
+Definition find_obj (id: ident) (menv: memoryEnv) : option memoryEnv :=
+  PM.find id (menv.(m_objects)).
 
 Definition constEnv : Set := PM.t const.
 
 Definition empty: constEnv := PM.empty const.
+Definition mempty: memoryEnv := mk_memory empty (PM.empty memoryEnv).
 
 Inductive exp_eval (menv: memoryEnv)(env: constEnv):
   exp -> const -> Prop :=
@@ -95,108 +87,6 @@ Inductive exp_eval (menv: memoryEnv)(env: constEnv):
     forall c ,
       exp_eval menv env (Const(c)) c.
 
-Inductive stmt_eval (menv: memoryEnv)(env: constEnv) :
-  stmt -> memoryEnv * constEnv -> Prop :=
-| Iassign:
-    forall x e v env',
-      exp_eval menv env e v ->
-      PM.add x v env = env' ->
-      stmt_eval menv env (Assign x e) (menv, env')
-| Iassignst:
-    forall x e v menv',
-      exp_eval menv env e v ->
-      add_mem x v menv = menv' ->
-      stmt_eval menv env (AssignSt x e) (menv', env)
-| Iapp:
-    forall e v o y env' s_fun res_value res_memory,
-      exp_eval menv env e v ->
-      find_object o menv = Some(s_fun) ->
-      application menv empty s_fun v (res_value, res_memory) ->
-      PM.add y res_value env  = env' ->
-      stmt_eval menv env (Step_ap y o e) (menv, env')
-| Icomp:
-    forall a1 a2 env1 menv1 env2 menv2,
-      stmt_eval menv env a1 (menv1, env1) ->
-      stmt_eval menv1 env1 a2 (menv2, env2) ->
-      stmt_eval menv env (Comp a1 a2) (menv2, env2)
-| Iifte_true:
-    forall b ifTrue ifFalse env' menv',
-      exp_eval menv env b (Cbool true) ->
-      stmt_eval menv env ifTrue (menv', env') ->
-      stmt_eval menv env (Ifte b ifTrue ifFalse) (menv', env')
-| Iifte_false:
-    forall b ifTrue ifFalse env' menv',
-      exp_eval menv env b (Cbool false) ->
-      stmt_eval menv env ifFalse (menv', env') ->
-      stmt_eval menv env (Ifte b ifTrue ifFalse) (menv', env')
-| Iskip:
-    stmt_eval menv env Skip (menv, env)
-
-with application (menv: memoryEnv)(env: constEnv) :
-       step_fun -> const -> const * memoryEnv -> Prop :=
-| Aapp:
-    forall s_fun arg_v v res_env res_memory,
-      stmt_eval menv (PM.add s_fun.(input) arg_v empty)
-           s_fun.(body) (res_memory, res_env) ->
-      PM.find s_fun.(output) res_env = Some(v) ->
-      application menv env s_fun arg_v (v, res_memory).
-
-Inductive run :
-  memoryEnv -> constEnv -> stmt -> nat -> memoryEnv * constEnv -> Prop :=
-| Run_empty:
-    forall menvInit envInit stmt,
-      run menvInit envInit stmt 0 (menvInit, envInit)
-| Run_cons:
-    forall menvInit menvInter menvFinal
-           envInit envInter envFinal
-           stmt n,
-      stmt_eval menvInit envInit stmt (menvInter, envInter) ->
-      run menvInter envInter stmt n (menvFinal, envFinal) ->
-      run menvInit envInit stmt (S n) (menvFinal, envFinal).
-
-
-Lemma stmt_eval_fold_left_shift:
-  forall A f (xs:list A) iacc menv env menv' env',
-    stmt_eval menv env
-              (List.fold_left (fun i x => Comp (f x) i) xs iacc)
-              (menv', env')
-    <->
-    exists menv'' env'',
-      stmt_eval menv env
-                (List.fold_left (fun i x => Comp (f x) i) xs Skip)
-                (menv'', env'')
-      /\
-      stmt_eval menv'' env'' iacc (menv', env').
-Proof.
-  Hint Constructors stmt_eval.
-  induction xs.
-  - split; [ now eauto | ].
-    intro H; do 2 destruct H.
-    destruct H as [H0 H1].
-    inversion_clear H0; apply H1.
-  - intros.
-    split.
-    + intro H0.
-      apply IHxs in H0.
-      destruct H0 as [menv'' H0].
-      destruct H0 as [env'' H0].
-      destruct H0 as [H0 H1].
-      inversion_clear H1.
-      exists menv1. exists env1.
-      split; try apply IHxs; eauto.
-    + intros;
-      repeat progress
-             match goal with
-             | H:exists _, _ |- _ => destruct H
-                  | H:_ /\ _ |- _ => destruct H
-             | H:stmt_eval _ _ (Comp _ Skip) _ |- _ => inversion_clear H
-             | H:stmt_eval _ _ Skip _ |- _ => inversion H; subst
-             | H:stmt_eval _ _ (List.fold_left _ _ _) _ |- _ => apply IHxs in H
-             | _ => eauto
-             end.
-      apply IHxs; eauto.
-Qed.
-
 Lemma exp_eval_det:
   forall menv env e v1 v2,
     exp_eval menv env e v1 ->
@@ -211,54 +101,249 @@ Proof.
     ( injection Hv2; trivial ) || apply Hv2.
 Qed.
 
-Lemma stmt_eval_det:
-  forall s menv env menv1 env1 menv2 env2,
-    stmt_eval menv env s (menv1, env1)
-    -> stmt_eval menv env s (menv2, env2)
-    -> menv2 = menv1 /\ env2 = env1.
-Proof.
-  induction s.
-  - intros menv env menv1 env1 menv2 env2 Hs1 Hs2.
-    inversion Hs1; inversion Hs2.
-    rewrite <- H7 in *.
-    rewrite <- H1 in *.
-    rewrite (exp_eval_det _ _ _ _ _ H8 H2) in *.
-    rewrite H10 in H4.
-    rewrite H4 in *.
-    intuition.
-  - intros menv env menv1 env1 menv2 env2 Hs1 Hs2.
-    inversion Hs1; inversion Hs2.
-    rewrite <- H3 in *.
-    rewrite <- H9 in *.
-    rewrite (exp_eval_det _ _ _ _ _ H8 H2) in *.
-    rewrite H10 in H4.
-    rewrite H4 in *.
-    intuition.
-  - intros menv env menv1 env1 menv2 env2 Hs1 Hs2.
-    inversion Hs1; inversion Hs2.
-    apply (IHs1 _ _ _ _ _ _ H5 H12).
-    discriminate (exp_eval_det _ _ _ _ _ H1 H8).
-    discriminate (exp_eval_det _ _ _ _ _ H1 H8).
-    apply (IHs2 _ _ _ _ _ _ H5 H12).
-  - intros menv env menv1 env1 menv2 env2 Hs1 Hs2.
-    inversion Hs1; inversion Hs2.
-    rewrite <- H11 in *.
-    rewrite <- H2 in *.
-    admit. (* TODO: handle node application *)
-  - intros menv env menv1 env1 menv2 env2 Hs1 Hs2.
-    inversion Hs1; inversion Hs2.
-    pose proof (IHs1 _ _ _ _ _ _ H2 H8) as HR.
-    destruct HR as [HR1 HR2].
-    rewrite HR1, HR2 in *.
-    pose proof (IHs2 _ _ _ _ _ _ H4 H10) as HR.
-    destruct HR as [HR3 HR4].
-    rewrite HR3, HR4 in *.
-    intuition.
-  - intros menv env menv1 env1 menv2 env2 Hs1 Hs2.
-    inversion Hs1; inversion Hs2.
-    rewrite <- H, <- H1, <- H0, <- H3.
-    intuition.
-Qed.
+Section stmt_eval.
+  Variable prog : program.
+
+  (* (* version: menv, env as parameters *)
+  Inductive stmt_eval (menv: memoryEnv) (env: constEnv) :
+    stmt -> memoryEnv * constEnv -> Prop :=
+  | Iassign:
+      forall x e v env',
+        exp_eval menv env e v ->
+        PM.add x v env = env' ->
+        stmt_eval menv env (Assign x e) (menv, env')
+  | Iassignst:
+      forall x e v menv',
+        exp_eval menv env e v ->
+        add_mem x v menv = menv' ->
+        stmt_eval menv env (AssignSt x e) (menv', env)
+  | Istep:
+      forall e v clsid cls o y menv' env' omenv omenv' rv,
+        find_class clsid prog = Some(cls) ->
+        find_obj o menv = Some(omenv) ->
+
+        exp_eval menv env e v ->
+        stmt_step_eval omenv (PM.add cls.(c_input) v empty) cls omenv' rv ->
+        add_obj o omenv' menv = menv' ->
+        PM.add y rv env  = env' ->
+        stmt_eval menv env (Step_ap y clsid o e) (menv', env')
+  | Ireset:
+      forall o clsid omenv' menv',
+        stmt_reset_eval mempty empty clsid omenv' ->
+        add_obj o omenv' menv = menv' ->
+        stmt_eval menv env (Reset_ap clsid o) (menv', env)
+  | Icomp:
+      forall a1 a2 env1 menv1 env2 menv2,
+        stmt_eval menv env a1 (menv1, env1) ->
+        stmt_eval menv1 env1 a2 (menv2, env2) ->
+        stmt_eval menv env (Comp a1 a2) (menv2, env2)
+  | Iifte_true:
+      forall b ifTrue ifFalse env' menv',
+        exp_eval menv env b (Cbool true) ->
+        stmt_eval menv env ifTrue (menv', env') ->
+        stmt_eval menv env (Ifte b ifTrue ifFalse) (menv', env')
+  | Iifte_false:
+      forall b ifTrue ifFalse env' menv',
+        exp_eval menv env b (Cbool false) ->
+        stmt_eval menv env ifFalse (menv', env') ->
+        stmt_eval menv env (Ifte b ifTrue ifFalse) (menv', env')
+  | Iskip:
+        stmt_eval menv env Skip (menv, env)
+  with stmt_step_eval (menv: memoryEnv) (env: constEnv) :
+         class -> memoryEnv -> const -> Prop :=
+  | Iestep:
+      forall ov cls menv' env',
+        stmt_eval menv env cls.(c_step) (menv', env') ->
+        PM.find cls.(c_output) env' = Some(ov) ->
+        stmt_step_eval menv env cls menv' ov
+  with stmt_reset_eval (menv: memoryEnv) (env: constEnv) :
+         ident -> memoryEnv -> Prop :=
+  | Iereset:
+      forall clsid cls menv' env',
+        find_class clsid prog = Some(cls) ->
+        stmt_eval menv env cls.(c_reset) (menv', env') ->
+        stmt_reset_eval menv env clsid menv'.
+   *)
+
+  Inductive stmt_eval :
+    memoryEnv -> constEnv -> stmt -> memoryEnv * constEnv -> Prop :=
+  | Iassign:
+      forall menv env x e v env',
+        exp_eval menv env e v ->
+        PM.add x v env = env' ->
+        stmt_eval menv env (Assign x e) (menv, env')
+  | Iassignst:
+      forall menv env x e v menv',
+        exp_eval menv env e v ->
+        add_mem x v menv = menv' ->
+        stmt_eval menv env (AssignSt x e) (menv', env)
+  | Istep:
+      forall menv env e v clsid o y menv' env' omenv omenv' rv,
+        find_obj o menv = Some(omenv) ->
+        exp_eval menv env e v ->
+        stmt_step_eval omenv clsid v omenv' rv ->
+        add_obj o omenv' menv = menv' ->
+        PM.add y rv env  = env' ->
+        stmt_eval menv env (Step_ap y clsid o e) (menv', env')
+  | Ireset:
+      forall menv env o clsid omenv' menv',
+        stmt_reset_eval clsid omenv' ->
+        add_obj o omenv' menv = menv' ->
+        stmt_eval menv env (Reset_ap clsid o) (menv', env)
+  | Icomp:
+      forall menv env a1 a2 env1 menv1 env2 menv2,
+        stmt_eval menv env a1 (menv1, env1) ->
+        stmt_eval menv1 env1 a2 (menv2, env2) ->
+        stmt_eval menv env (Comp a1 a2) (menv2, env2)
+  | Iifte_true:
+      forall menv env b ifTrue ifFalse env' menv',
+        exp_eval menv env b (Cbool true) ->
+        stmt_eval menv env ifTrue (menv', env') ->
+        stmt_eval menv env (Ifte b ifTrue ifFalse) (menv', env')
+  | Iifte_false:
+      forall menv env b ifTrue ifFalse env' menv',
+        exp_eval menv env b (Cbool false) ->
+        stmt_eval menv env ifFalse (menv', env') ->
+        stmt_eval menv env (Ifte b ifTrue ifFalse) (menv', env')
+  | Iskip:
+      forall menv env,
+        stmt_eval menv env Skip (menv, env)
+  with stmt_step_eval :
+         memoryEnv -> ident -> const -> memoryEnv -> const -> Prop :=
+  | Iestep:
+      forall menv clsid iv menv' ov cls env',
+        find_class clsid prog = Some(cls) ->
+        stmt_eval menv (PM.add cls.(c_input) iv empty) cls.(c_step)
+                  (menv', env') ->
+        PM.find cls.(c_output) env' = Some(ov) ->
+        stmt_step_eval menv clsid iv menv' ov
+  with stmt_reset_eval : ident -> memoryEnv -> Prop :=
+  | Iereset:
+      forall clsid cls menv' env',
+        find_class clsid prog = Some(cls) ->
+        stmt_eval mempty empty cls.(c_reset) (menv', env') ->
+        stmt_reset_eval clsid menv'.
+
+  Scheme stmt_eval_mult := Induction for stmt_eval Sort Prop
+  with stmt_step_eval_mult := Induction for stmt_step_eval Sort Prop
+  with stmt_reset_eval_mult := Induction for stmt_reset_eval Sort Prop.
+
+  Inductive run :
+    memoryEnv -> constEnv -> stmt -> nat -> memoryEnv * constEnv -> Prop :=
+  | Run_empty:
+      forall menvInit envInit stmt,
+        run menvInit envInit stmt 0 (menvInit, envInit)
+  | Run_cons:
+      forall menvInit menvInter menvFinal
+             envInit envInter envFinal
+             stmt n,
+        stmt_eval menvInit envInit stmt (menvInter, envInter) ->
+        run menvInter envInter stmt n (menvFinal, envFinal) ->
+        run menvInit envInit stmt (S n) (menvFinal, envFinal).
+
+  Lemma stmt_eval_fold_left_shift:
+    forall A f (xs:list A) iacc menv env menv' env',
+      stmt_eval menv env
+                (List.fold_left (fun i x => Comp (f x) i) xs iacc)
+                (menv', env')
+      <->
+      exists menv'' env'',
+        stmt_eval menv env
+                  (List.fold_left (fun i x => Comp (f x) i) xs Skip)
+                  (menv'', env'')
+        /\
+        stmt_eval menv'' env'' iacc (menv', env').
+  Proof.
+    Hint Constructors stmt_eval.
+    induction xs.
+    - split; [ now eauto | ].
+      intro H; do 2 destruct H.
+      destruct H as [H0 H1].
+      inversion_clear H0; apply H1.
+    - intros.
+      split.
+      + intro H0.
+        apply IHxs in H0.
+        destruct H0 as [menv'' H0].
+        destruct H0 as [env'' H0].
+        destruct H0 as [H0 H1].
+        inversion_clear H1.
+        exists menv1. exists env1.
+        split; try apply IHxs; eauto.
+      + intros;
+        repeat progress
+             match goal with
+             | H:exists _, _ |- _ => destruct H
+             | H:_ /\ _ |- _ => destruct H
+             | H:stmt_eval _ _ (Comp _ Skip) _ |- _ => inversion_clear H
+             | H:stmt_eval _ _ Skip _ |- _ => inversion H; subst
+             | H:stmt_eval _ _ (List.fold_left _ _ _) _ |- _ => apply IHxs in H
+             | _ => eauto
+             end.
+        apply IHxs; eauto.
+  Qed.
+
+  Lemma stmt_eval_det:
+    forall s menv env renv1 renv2,
+      stmt_eval menv env s renv1
+      -> stmt_eval menv env s renv2
+      -> renv1 = renv2.
+  Proof.
+    intros s menv env renv1 renv2 Hs1.
+    revert renv2.
+    induction Hs1 using stmt_eval_mult
+    with (P:=fun menv env s renv1 sev=>
+               forall renv2, stmt_eval menv env s renv2 -> renv1 = renv2)
+         (P0:=fun menv clsid v menv' rv ssev=>
+                forall menv'' rv', stmt_step_eval menv clsid v menv'' rv'
+                                   -> menv' = menv'' /\ rv = rv')
+         (P1:=fun i menv srev=>
+                forall menv', stmt_reset_eval i menv' -> menv = menv');
+      inversion_clear 1;
+      repeat progress match goal with
+      | Ht: exp_eval ?menv ?env ?e (Cbool true),
+        Hf: exp_eval ?menv ?env ?e (Cbool false) |- _ =>
+        pose proof (exp_eval_det _ _ _ _ _ Ht Hf) as Hneq; discriminate
+      | H1:exp_eval ?menv ?env ?e ?v1,
+        H2:exp_eval ?menv ?env ?e ?v2 |- _ =>
+        pose proof (exp_eval_det _ _ _ _ _ H1 H2) as Heq;
+          rewrite Heq in *; clear Heq H1 H2
+      | H1: PM.add ?x ?v ?env = ?env1,
+        H2: PM.add ?x ?v ?env = ?env2 |- _ =>
+        rewrite H1 in H2; rewrite H2 in *; clear H1 H2
+      | H1: add_mem ?x ?v ?menv = ?menv1,
+        H2: add_mem ?x ?v ?menv = ?menv2 |- _ =>
+        rewrite H1 in H2; rewrite H2 in *; clear H1 H2
+      | H1: find_obj ?o ?menv = Some ?omenv1,
+        H2: find_obj ?o ?menv = Some ?omenv2 |- _ =>
+        rewrite H1 in H2; injection H2; intro Heq; rewrite Heq in *;
+        clear H1 H2 Heq
+      | H1: find_class ?clsid ?prog = _,
+        H2: find_class ?clsid ?prog = _ |- _ =>
+        rewrite H1 in H2; injection H2;
+        intro Heq; rewrite Heq in *; clear H2 H2
+      | H1: PM.find ?x ?env = ?rv1,
+        H2: PM.find ?x ?env = ?rv2 |- _ =>
+        rewrite H1 in H2; injection H2; rewrite H2 in *; clear H1 H2
+      | Hs: stmt_step_eval ?omenv ?clsid ?v _ _,
+        IH: context[stmt_step_eval ?omenv ?clsid ?v _ _ -> _ = _ /\ _ = _] |- _ =>
+        apply IH in Hs; destruct Hs as [Heq1 Heq2]; try rewrite Heq1 in *;
+        try rewrite Heq2 in *; clear Heq1 Heq2
+      | Hs: stmt_reset_eval ?clsid _,
+        IH: context[stmt_reset_eval ?clsid _ -> _ = _] |- _ =>
+        apply IH in Hs; try rewrite Hs in *; clear Hs
+      | Hs: stmt_eval ?menv ?env ?stmt _,
+        IH: context[stmt_eval ?menv ?env ?stmt _ -> (_, _) = _] |- _ =>
+        apply IH in Hs; injection Hs; intros Heq1 Heq2;
+        try rewrite Heq1 in *; try rewrite Heq2 in *; clear Heq1 Heq2 Hs
+      | H1: add_obj ?o ?omenv ?menv = ?menv1,
+        H2: add_obj ?o ?omenv ?menv = ?menv2 |- _ =>
+        rewrite H1 in H2; rewrite H2 in *; clear H1 H2
+      | _ => intuition
+      end.
+  Qed.
+
+End stmt_eval.
 
 Lemma find_mem_gss:
   forall y c m, find_mem y (add_mem y c m) = Some c.
@@ -271,5 +356,4 @@ Lemma find_mem_gso:
 Proof.
   intros. apply PM.gso. assumption.
 Qed.
-
 
