DataflowNatMSemantics.v
@@ -1,0 +1,494 @@
+Require Import Coq.FSets.FMapPositive.
+Require Import Rustre.Common.
+Require Import Rustre.DataflowSyntax.
+Require Import SynchronousNat.
+Require Import DataflowNatSemantics.
+
+(*
+   NB: The history H is not really necessary here. We could just as well
+       replay all the semantic definitions using a valueEnv N ('N' for now),
+       since all the historical information is in ms. This approach would
+       have two advantages:
+
+       1. Conceptually cleanliness: N corresponds more or less to the
+          temporary variables in the Minimp implementation (except that it
+          would also contain values for variables defined by EqFby).
+
+       2. No index needed to access values in when reasoning about
+          translation correctness.
+
+       But this approach requires more uninteresting definitions and
+       and associated proofs of properties, and a longer proof of equivalence
+       with sem_node: too much work for too little gain.
+ *)
+
+Inductive memory : Set := mk_memory {
+  mm_values : PM.t (nat -> const);
+  mm_instances : PM.t memory
+}.
+
+Definition mfind_mem x menv := PM.find x menv.(mm_values).
+Definition mfind_inst f menv := PM.find f menv.(mm_instances).
+
+Inductive msem_equation (G: global) : history -> memory -> equation -> Prop :=
+| SEqDef:
+    forall H M x cae,
+      (forall n,
+          exists v, sem_var H x n v
+                    /\ sem_caexp H cae n v) ->
+      msem_equation G H M (EqDef x cae)
+| SEqApp:
+    forall H M x f M' arg,
+      mfind_inst f M = Some M' ->
+      (forall ls xs,
+          (forall n, sem_laexp H arg n (ls n)) ->
+          (forall n, sem_var H x n (xs n)) ->
+          msem_node G f ls M' xs) ->
+      msem_equation G H M (EqApp x f arg)
+| SEqFby:
+    forall H M ms x ls v0 lae,
+      mfind_mem x M = Some ms ->
+      ms 0 = v0 ->
+      (forall n, sem_laexp H lae n (ls n)) ->
+      (forall n, match ls n with
+                 | absent    => ms (S n) = ms n              (* held *)
+                                /\ sem_var H x n absent
+                 | present v => ms (S n) = v
+                                /\ sem_var H x n (present (ms n))
+                 end) ->
+      msem_equation G H M (EqFby x v0 lae)
+
+with msem_node (G: global) : ident -> stream -> memory -> stream -> Prop :=
+| SNode:
+    forall f xs M ys i o eqs,
+      find_node f G = Some (mk_node f i o eqs) ->
+      (exists (H: history),
+        (forall n, sem_var H i.(v_name) n (xs n))
+        /\ (forall n, sem_var H o.(v_name) n (ys n))
+        /\ List.Forall (msem_equation G H M) eqs) ->
+        msem_node G f xs M ys.
+
+(* TODO: Warning: Ignoring recursive call
+         We must write these induction principles manually. *)
+(*
+Scheme msem_equation_mult := Induction for msem_equation Sort Prop
+with msem_node_mult := Induction for msem_node Sort Prop.
+
+(* TODO: move to DataflowNatSemantics.v *)
+Scheme sem_equation_mult := Induction for sem_equation Sort Prop
+with sem_node_mult := Induction for sem_node Sort Prop.
+*)
+
+Definition msem_nodes (G: global) : Prop :=
+  List.Forall (fun no => exists xs M ys, msem_node G no.(n_name) xs M ys) G.
+
+(* TODO:
+    show that:
+       sem_node G f xs ys
+       <->
+       (exists ms, msem_node G f xs ms ys)
+
+    this requires constructing an ms: what can we reuse from the
+    sem_held_equations development?
+
+    then it is trivial that:
+       sem_nodes G <-> msem_nodes G
+ *)
+
+
+Lemma sem_msem_node:
+  forall G f xs ys,
+    sem_node G f xs ys <-> (exists ms, msem_node G f xs ms ys).
+Proof.
+  intros G f xs ys.
+  split; [ intro Hsem | intro Hmsem ].
+  - admit.
+  - admit.
+Qed.
+
+(* TODO:
+    - rework is_step_correct.
+    - base it on msem_node G f xs ms ys
+    - induction on G, with well-defined predicate
+    - memories correspond to values of ms (and recursively for called nodes)
+    - local history corresponds to env
+    - inputs and outputs link correctly with xs and ys
+
+    - show that reset gives the first memory
+ *)
+
+(* TODO:
+    - prove correctness in terms of sem_node G f xs ys,
+      hiding the internal memory details.
+      (provided the initial memory is created by reset)
+ *)
+
+(* TODO: Replace with the new development in DataflowNatMSemantics:
+
+Inductive sem_held_equation (H: history) (H': history) : equation -> Prop :=
+| SHEqDef:
+    forall x cae,
+      (forall n c, sem_var H x n (present c) -> sem_var H' x n (present c))
+      -> sem_held_equation H H' (EqDef x cae)
+| SHEqApp:
+    forall x f lae,
+      (forall n c, sem_var H x n (present c) -> sem_var H' x n (present c))
+      -> sem_held_equation H H' (EqApp x f lae)
+| SHEqFby:
+    forall x v0 lae ys,
+      (forall n, sem_laexp H lae n (ys n))
+      -> (forall n c, sem_var H' x n (present c) <-> holdR v0 ys n c)
+      -> sem_held_equation H H' (EqFby x v0 lae).
+
+Definition sem_held_equations
+           (H: history) (H': history) (eqs: list equation) : Prop :=
+  List.Forall (sem_held_equation H H') eqs.
+
+Lemma sem_held_equations_tl:
+  forall H H' eq eqs,
+    sem_held_equations H H' (eq::eqs) -> sem_held_equations H H' eqs.
+Proof.
+  intros H H' eq eqs Hsem.
+  apply Forall_cons2 in Hsem.
+  intuition.
+Qed.
+
+Lemma sem_held_equations_corres:
+  forall G H H' eqs,
+    sem_equations G H eqs
+    -> sem_held_equations H H' eqs
+    -> (forall x n c,
+           Is_defined_in x eqs
+           -> sem_var H x n (present c)
+           -> sem_var H' x n (present c)).
+Proof.
+  induction eqs as [|eq]; [inversion 3|].
+  intros Hs Hsh x n c Hdef Hsv.
+  apply Forall_cons2 in Hs; destruct Hs as [Hseq Hseqs];
+  apply Forall_cons2 in Hsh; destruct Hsh as [Hsheq Hsheqs];
+  apply Is_defined_in_cons in Hdef; destruct Hdef as [Hdef|Hdef];
+  [ | destruct Hdef as [Hndef Hdef];
+      apply (IHeqs Hseqs Hsheqs _ _ _ Hdef Hsv) ].
+  destruct eq as [| |y v0 lae]; inversion Hdef; subst;
+  inversion_clear Hsheq as [? ? HH|? ? ? HH|? ? ? ys Hys HH];
+  apply HH; try apply Hsv.
+
+  inversion_clear Hseq as [| |? xs ? ? Hxs Hfby].
+  rewrite sem_laexp_repr in Hxs.
+  assert (forall n, xs n = ys n) as Hxsys by
+        (intro n0;
+         specialize Hys with n0;
+         specialize Hxs with n0 (xs n0);
+         apply sem_laexp_det with H n0 lae;
+         (apply Hxs; reflexivity) || apply Hys).
+  apply Hfby in Hsv.
+  rewrite <- (holdR_ext _ _ Hxsys).
+  apply fbyR_holdR with (1:=Hsv).
+Qed.
+
+Section StreamGenerators.
+
+  Variable H: history.
+  Variable arbitrary : stream.
+
+  Definition const_eqb (c1: const) (c2: const) : bool :=
+    match (c1, c2) with
+    | (Cint z1, Cint z2) => BinInt.Z.eqb z1 z2
+    | (Cbool b1, Cbool b2) => Bool.eqb b1 b2
+    | _ => false
+    end.
+
+  Definition value_eqb (v1: value) (v2: value) : bool :=
+    match (v1, v2) with
+    | (present c1, present c2) => const_eqb c1 c2
+    | (absent, absent) => true
+    | _ => false
+    end.
+
+  Fixpoint str_clock (ck: clock) (n: nat) : bool :=
+    match ck with
+    | Cbase => true
+    | Con ck' x c => match PM.find x H with
+                     | None => false
+                     | Some xs => andb (str_clock ck' n)
+                                       (value_eqb (xs n) (present (Cbool c)))
+                     end
+    end.
+
+  Fixpoint str_lexp (e: lexp) (n: nat) : value :=
+    match e with
+    | Econst c => present c
+    | Evar x => match PM.find x H with
+                | Some xs => xs n
+                | None => absent
+                end
+    | Ewhen e' x c => match PM.find x H with
+                      | Some xs => match xs n with
+                                   | present (Cbool b) =>
+                                     if Bool.eqb b c
+                                     then str_laexp e' n
+                                     else absent
+                                   | _ => absent
+                                   end
+                      | None => absent
+                      end
+    end
+  with str_laexp (e: laexp) (n: nat) : value :=
+    match e with
+    | LAexp ck e => if str_clock ck n then str_lexp e n else absent
+    end.
+
+  Lemma str_clock_spec:
+    forall ck n c,
+      sem_clock H ck n c
+      -> str_clock ck n = c.
+  Proof.
+    induction ck.
+    inversion 1; intuition.
+    intros n c.
+    inversion_clear 1;
+      repeat progress (simpl;
+         match goal with
+         | H:sem_var _ _ _ _ |- _ => inversion_clear H
+         | H: PM.find _ _ = _ |- _ => rewrite H
+         | H: _ = present (Cbool ?b) |- _ => (rewrite H; destruct b)
+         | H: sem_clock _ _ _ _ |- _ => (apply IHck in H; rewrite H)
+         | H: b <> _ |- _ => (apply Bool.not_true_is_false in H
+                              || apply Bool.not_false_is_true in H;
+                              rewrite H)
+         | _ => (cbv; reflexivity)
+         end).
+    destruct (PM.find i H); cbv; reflexivity.
+  Qed.
+
+  Lemma str_lexp_spec:
+    forall e n v,
+      sem_lexp H e n v
+      -> str_lexp e n = v.
+  Proof.
+    induction e using lexp_mult
+    with (P:=fun e => forall n v, sem_laexp H e n v -> str_laexp e n = v);
+    inversion 1;
+    repeat progress (simpl;
+           match goal with
+           | H:sem_lexp _ _ _ _ |- _ => (apply IHe in H; rewrite H)
+           | H:sem_laexp _ _ _ _ |- _ => (apply IHe in H; rewrite H)
+           | H:sem_clock _ _ _ _ |- _ => (apply str_clock_spec in H; rewrite H)
+           | H:sem_var _ _ _ _ |- _ => (inversion_clear H as [xs Hfind Hxsn];
+                                        rewrite Hfind; rewrite Hxsn)
+           | |- (if Bool.eqb ?b1 ?b2 then _ else _) = _ =>
+             try destruct b1; try destruct b2; simpl; intuition
+           | _ => intuition
+           end).
+  Qed.
+
+  Lemma str_laexp_spec:
+    forall e n v,
+      sem_laexp H e n v
+      -> str_laexp e n = v.
+  Proof.
+    inversion_clear 1; simpl;
+    repeat progress
+           match goal with
+           | H:sem_clock _ _ _ _ |- _ => (apply str_clock_spec in H; rewrite H)
+           | H:sem_lexp _ _ _ _ |- _ => (apply str_lexp_spec in H; rewrite H)
+           | _ => intuition
+           end.
+  Qed.
+
+End StreamGenerators.
+
+Definition hold_history (H: history) : history -> list equation -> history :=
+  List.fold_right
+    (fun eq H' =>
+       match eq with
+       | EqFby x v0 e => PM.add x (fun n=>present (hold v0 (str_laexp H e) n)) H'
+       | EqApp x _ _ => H'
+       | EqDef x _ => H'
+       end).
+
+(* An alternative lemma would be:
+   sem_held_equations H H' (filter_dup_defs eqs) -> sem_held_equations H H' eqs
+   which should hold since the H in sem_equations/sem_held_equations requires
+   that multiple definitions of the same variable be coherent. But proving
+   this stronger result is much harder than just assuming something that
+   should anyway be true: there are no duplicate definitions in eqs.
+
+   Note, however, that this requires a stronger definition of Is_well_sch. *)
+Lemma not_in_add_to_sem_held_equations:
+  forall x xs eqs H H',
+    ~Is_defined_in x eqs
+    -> sem_held_equations H H' eqs
+    -> sem_held_equations H (PM.add x xs H') eqs.
+Proof.
+  induction eqs as [|eq].
+  intuition (apply List.Forall_nil).
+  intros H H' Hndef Hsem.
+  apply not_Is_defined_in_cons in Hndef; destruct Hndef as [Hndef0 Hndef1].
+  unfold sem_held_equations in Hsem.
+  apply Forall_cons2 in Hsem; destruct Hsem as [Hsem0 Hsem1].
+  apply (IHeqs _ _ Hndef1) in Hsem1.
+  destruct eq; [ apply not_Is_defined_in_eq_EqDef in Hndef0
+               | apply not_Is_defined_in_eq_EqApp in Hndef0
+               | apply not_Is_defined_in_eq_EqFby in Hndef0 ];
+  apply List.Forall_cons; try apply Hsem1;
+  inversion_clear Hsem0 as [? ? Hsv|? ? ? Hsv|? ? ? ys Hlae Hsv];
+  try constructor;
+  intros;
+  try (apply sem_var_gso with (1:=Hndef0); apply Hsv; assumption).
+  apply SHEqFby with (1:=Hlae).
+  intros; rewrite <- Hsv; split; intro HH.
+  apply sem_var_gso with (1:=Hndef0) in HH; assumption.
+  apply sem_var_gso with (1:=Hndef0); assumption.
+Qed.
+
+
+(*
+   eqs = [ EqDef x y; EqFby y (Cint 0) (Econst (Cint 1)) ]
+   eqs' = eqFby x (Cint 0) (Econst (Cint 1)) :: eqs
+
+   Both eqs and eqs' have a coherent semantics (sem_equations G H _),
+   but their respective hold semantics differ (for eqs', x is always present).
+*)
+Lemma sem_held_equations_existence:
+  forall G H eqs,
+    sem_equations G H eqs
+    -> no_dup_defs eqs
+    -> sem_held_equations H (hold_history H H eqs) eqs
+       /\ (forall y n c,
+              sem_var H y n (present c)
+              -> sem_var (hold_history H H eqs) y n (present c)).
+Proof.
+  intros G H eqs Hsem Hndups.
+  induction eqs as [|eq].
+  - intuition constructor.
+  - apply Forall_cons2 in Hsem; destruct Hsem as [Hsem Hsems].
+    apply IHeqs in Hsems; [clear IHeqs
+                          | inversion_clear Hndups; assumption ].
+    destruct Hsems as [Hsems Hvars].
+    destruct eq.
+
+    split; [apply Forall_cons2|intuition];
+    split; [constructor; apply Hvars|intuition].
+
+    split; [apply Forall_cons2|intuition];
+    split; [constructor; apply Hvars|intuition].
+
+    split.
+
+    (* show: sem_var -> sem_var *)
+    Focus 2.
+    intros y n c0 Hvar.
+    pose proof (Hvars _ _ _ Hvar) as Hvar'.
+    destruct (ident_eq_dec i y) as [Hiy|Hniy]; [rewrite Hiy|].
+    2:(inversion_clear Hvar'; apply Sv with xs; simpl; try rewrite PM.gso; auto).
+    simpl.
+    eapply Sv.
+    rewrite PM.gss.
+    rewrite <-Some_injection.
+    reflexivity.
+    simpl.
+    apply present_injection.
+    inversion_clear Hsem.
+    rewrite Hiy in *.
+    apply H1 in Hvar.
+    rewrite hold_injection with _ xs _ _.
+    apply hold_rel.
+    apply fbyR_holdR.
+    exact Hvar.
+    intro n0.
+    rewrite sem_laexp_repr in H0.
+    specialize H0 with n0 (xs n0).
+    assert (sem_laexp H l n0 (xs n0)) as Hsl by (apply H0; reflexivity).
+    apply str_laexp_spec in Hsl.
+    exact Hsl.
+
+    (* show sem_held_equations *)
+
+    simpl.
+    apply Forall_cons2.
+    split.
+    inversion_clear Hsem.
+    apply SHEqFby with xs.
+    apply H0.
+    intros n c0.
+    split.
+    inversion_clear 1.
+    rewrite PM.gss in H3.
+    injection H3.
+    intro.
+    rewrite <-H2 in H4.
+    injection H4.
+    intro.
+    apply hold_rel.
+    rewrite <-H5.
+    apply hold_injection.
+    intro n0.
+    specialize H0 with n0.
+    apply str_laexp_spec in H0.
+    rewrite H0.
+    reflexivity.
+    intro Hhold.
+    apply hold_rel in Hhold.
+    eapply Sv.
+    rewrite PM.gss.
+    rewrite <-Some_injection.
+    reflexivity.
+    simpl.
+    apply present_injection.
+    rewrite hold_injection with _ xs _ _.
+    apply Hhold.
+    intro n0.
+    specialize H0 with n0.
+    apply str_laexp_spec in H0.
+    exact H0.
+
+    apply not_in_add_to_sem_held_equations.
+    inversion_clear Hndups as [|? ? Hndups'].
+    apply Hndups'.
+    constructor.
+    apply Hsems.
+Qed.
+
+Lemma sem_held_equations_exist:
+  forall G H eqs,
+    sem_equations G H eqs
+    -> no_dup_defs eqs
+    -> exists H', sem_held_equations H H' eqs.
+Proof.
+  intros H H' eqs Hsems Hndups.
+  apply sem_held_equations_existence in Hsems.
+  destruct Hsems as [Hsems].
+  now (eexists; apply Hsems).
+  assumption.
+Qed.
+
+Lemma sem_equations_app2:
+  forall G H oeqs eqs,
+    sem_equations G H (oeqs ++ eqs)
+    -> sem_equations G H eqs.
+Proof.
+  intros G H oeqs eqs H0.
+  apply Forall_app in H0; intuition.
+Qed.
+
+Lemma sem_held_equations_app2:
+  forall H H' oeqs eqs,
+    sem_held_equations H H' (oeqs ++ eqs)
+    -> sem_held_equations H H' eqs.
+Proof.
+  intros H H' oeqs eqs H0.
+  apply Forall_app in H0; intuition.
+Qed.
+
+Lemma sem_held_equations_cons:
+  forall H H' eq eqs,
+    sem_held_equations H H' (eq :: eqs)
+    <-> sem_held_equation H H' eq /\ sem_held_equations H H' eqs.
+Proof.
+  split; intro Hs.
+  apply Forall_cons2 in Hs; auto.
+  apply Forall_cons2; auto.
+Qed.
+*)
+
